Splinter/Betree/Buffers.i.dfy
@@ -1,0 +1,68 @@
+// Copyright 2018-2021 VMware, Inc., Microsoft Inc., Carnegie Mellon University, ETH Zurich, and University of Washington
+// SPDX-License-Identifier: BSD-2-Clause
+
+include "../../lib/Base/KeyType.s.dfy"
+include "../../Spec/Message.s.dfy"
+
+module Buffers
+{
+  import opened KeyType
+  import opened ValueMessage
+
+  // I'd prefer to instantiate TotalMapMod here, but rank_is_less_than doesn't
+  // make it through the module refinement, so I can't prove decreases when I
+  // recursively walk down the BetreeNode. So I do it manually instead.
+  predicate AnyKey(key: Key) { true }
+  predicate Total(keys: iset<Key>) {
+    forall k | AnyKey(k) :: k in keys
+  }
+  function AllKeys() : (out: iset<Key>)
+    ensures Total(out)
+  {
+    iset k | AnyKey(k)
+  }
+
+  datatype Buffer = Buffer(mapp: map<Key, Message>)
+  {
+    function Query(key: Key) : Message
+    {
+      if key in mapp then mapp[key] else Update(NopDelta())
+    }
+
+    function ApplyFilter(accept: iset<Key>) : Buffer
+    {
+      Buffer(map k | k in mapp && k in accept :: mapp[k])
+    }
+  }
+
+  // buffers[0] is the newest data
+  datatype BufferStack = BufferStack(buffers: seq<Buffer>)
+  {
+    function QueryUpTo(key: Key, count: nat) : Message
+      requires count <= |buffers|
+    {
+      if count == 0 then Update(NopDelta())
+      else Merge(QueryUpTo(key, count-1), buffers[count-1].Query(key))
+    }
+
+    function Query(key: Key) : Message
+    {
+      QueryUpTo(key, |buffers|)
+    }
+
+    function ApplyFilter(accept: iset<Key>) : BufferStack
+    {
+      BufferStack(seq(|buffers|, i requires 0<=i<|buffers| => buffers[i].ApplyFilter(accept)))
+    }
+
+    function PrependBufferStack(newBuffers: BufferStack) : BufferStack
+    {
+      BufferStack(newBuffers.buffers + this.buffers)
+    }
+
+    predicate Equivalent(other: BufferStack)
+    {
+      forall k | AnyKey(k) :: Query(k) == other.Query(k)
+    }
+  }
+}
