Splinter/Betree/Memtable.i.dfy
@@ -1,0 +1,52 @@
+// Copyright 2018-2021 VMware, Inc., Microsoft Inc., Carnegie Mellon University, ETH Zurich, and University of Washington
+// SPDX-License-Identifier: BSD-2-Clause
+
+include "../../lib/Base/KeyType.s.dfy"
+include "../../Spec/Message.s.dfy"
+include "../CoordinationLayer/MsgHistory.i.dfy"
+
+module MemtableMod
+{
+  import opened KeyType
+  import opened ValueMessage
+  import opened LSNMod
+  import opened MsgHistoryMod
+
+  datatype Memtable = Memtable(mapp: map<Key, Message>, seqEnd: LSN)
+  {
+    function Get(key: Key) : Message
+    {
+      if key in mapp then mapp[key] else Update(NopDelta())
+    }
+
+    function ApplyPut(km: KeyedMessage) : Memtable
+    {
+      Memtable(mapp[km.key := Merge(km.message, Get(km.key))], seqEnd+1)
+    }
+
+    function ApplyPuts(puts: MsgHistory) : Memtable
+      requires puts.WF()
+      requires puts.seqStart == seqEnd
+      decreases puts.Len()
+    {
+      if puts.IsEmpty() then this
+      else ApplyPuts(puts.DiscardRecent(puts.seqEnd-1)).ApplyPut(puts.msgs[puts.seqEnd-1])
+    }
+
+    function Query(key: Key) : Message
+    {
+      if key in mapp then mapp[key] else Update(NopDelta())
+    }
+
+    // Drain out the contents (into the StampedBetree), but remember the seqEnd
+    function Drain() : Memtable
+    {
+      EmptyMemtable(seqEnd)
+    }
+  }
+
+  function EmptyMemtable(lsn: LSN) : Memtable
+  {
+    Memtable(map[], lsn)
+  }
+}
